

ash

## 1 562 to 567

[Stirling's approximation]

$$n! = \sqrt{2\pi n} \left(\frac{n}{e}\right)^n e^{r_n}$$

여기서  $r_n$ 은 다음 부등식을 만족한다.

$$\frac{1}{12n+1} < r_n < \frac{1}{12n}$$

*Proof.* Let

$$S_n = \log(n!) = \sum_{p=1}^{n-1} \log(p+1)$$

and write

$$\log(p+1) = A_p + b_p - \epsilon_p$$

where

$$\begin{aligned} A_p &= \int_p^{p+1} \log x \, dx, \\ b_p &= \frac{1}{2} (\log(p+1) - \log p), \\ \epsilon_p &= \int_p^{p+1} \log x \, dx - \frac{1}{2} [\log(p+1) + \log p]. \end{aligned}$$

then

$$\begin{aligned} S_n &= \sum_{p=1}^{n-1} (A_p + b_p - \epsilon_p) = \int_1^n \log(x) dx + \frac{1}{2} \log(n) - \sum_{p=1}^{n-1} \epsilon_p \\ &= (n + \frac{1}{2} \log(n) - n + 1) - \sum_{p=1}^{n-1} \epsilon_p, \\ \epsilon_p &= \frac{2p+1}{2} \log\left(\frac{p+1}{p}\right) - 1. \end{aligned}$$

using Taylor expansion of  $\log(1+x)$ , we have

$$\log\left(\frac{1+x}{1-x}\right) = 2\left(x + \frac{x^3}{3} + \frac{x^5}{5} + \cdots\right)$$

valid for  $|x| < 1$ , let  $x = (2p+1)^{-1}$ , so that  $\frac{1+x}{1-x} = \frac{p+1}{p}$ .

$$\epsilon_p = \frac{1}{3(2p+1)^2} + \frac{1}{5(2p+1)^4} + \cdots$$

**Upper bound of  $\epsilon_p$ :**

Since the coefficients decrease ( $\frac{1}{3} > \frac{1}{5} > \frac{1}{7} > \cdots$ ),

$$\begin{aligned}\epsilon_p &< \frac{1}{3}x^2(1+x^2+x^4+\cdots) \\ &= \frac{x^2}{3} \cdot \frac{1}{1-x^2} = \frac{1}{12}\left(\frac{1}{p} - \frac{1}{p+1}\right)\end{aligned}$$

**lower bound of  $\epsilon_p$ :**

$$\epsilon_p > \frac{x^2}{3}\left(1 + \frac{x^2}{3} + \frac{x^4}{3^2}\right) = \frac{x^2}{3} \cdot \frac{1}{1 - \frac{x^2}{3}} = \frac{1}{12p^2 + 12p + 2} > \frac{1}{12p^2 + 14p + \frac{13}{12}}$$

rewrite:

$$\begin{aligned}\sum_{p=1}^{n-1} \epsilon_p &= \underbrace{\sum_{p=1}^{\infty} \epsilon_p}_B - \underbrace{\sum_{p=n}^{\infty} \epsilon_p}_{r_n} \\ \frac{1}{13} &< B < \frac{1}{12} \\ \frac{1}{12n+1} &< r_n < \frac{1}{12n}\end{aligned}$$

rewrite  $S_n$ :

$$S_n = \left(n + \frac{1}{2}\right) \log n - n + 1 - B + r_n$$

so,

$$\begin{aligned}n! &= e^{S_n} \\ &= e^{1-B} \cdot n^{n+\frac{1}{2}} e^{-n} \cdot e^{r_n}\end{aligned}$$

and  $e^{1-B} = \sqrt{2\pi}$ .

□

## 2 CLT

**Theorem 1** (Central Limit Theorem). *assume that the random variables  $X_1, X_2, \dots$  are i.i.d with expectation  $\mu$  and variance  $\sigma^2$ . Then:*

$$P\left(\frac{X_1 + X_2 + \dots + X_n - \mu n}{\sigma\sqrt{n}} \leq x\right) \rightarrow P(Z \leq x)$$

*Proof.* let

$$T_n = \frac{S_n - n\mu}{\sigma\sqrt{n}}$$

we will show  $\phi_{T_n}(t) \rightarrow \phi_Z(t)$ .

let  $Y_i = \frac{X_i - \mu}{\sigma}$ , then  $E[Y_i] = 0$ ,  $Var(Y_i) = 1$

$$\begin{aligned}\phi_{T_n}(t) &= E[e^{tT_n}] \\&= E\left[e^{\frac{t}{\sqrt{n}}Y_1 + \dots + Y_n}\right] \\&= E\left[e^{\frac{t}{\sqrt{n}}Y}\right]^n \\&= E\left[1 + \frac{t}{\sqrt{n}}Y + \frac{t^2}{2n}Y^2 + \dots\right]^n \\&= E\left[1 + 0 + \frac{t^2}{2n}Y^2\right]^n \\&= \left(1 + \frac{t^2}{2n}E[Y^2]\right)^n \\&= \left(1 + \frac{t^2}{2n}\right)^n && \text{since } E[Y^2] = Var[Y] + (E[Y])^2 \\&= e^{\frac{t^2}{2}} \quad \text{as } n \rightarrow \infty \\&= \phi_Z(t)\end{aligned}$$

□

## 3 Markov Chain